extension to generalized axioms

coq.yalla/cokada.v
@@ -1,4 +1,5 @@
-Require Import List_more Permutation_Type genperm_Type.
+Require Import Psatz.
+Require Import List_more List_Type_more Permutation_Type genperm_Type wf_nat_more.
 
 Require Import closure_operators cphase_sem.
 
@@ -9,8 +10,320 @@ Notation "X '≃' Y" := (eqset X Y) (at level 75, format "X  ≃  Y", no associa
 Notation "A '∩' B" := (fun z => A z * B z : Type)%type (at level 50, format "A  ∩  B", left associativity).
 Notation "A '∪' B" := (fun z => A z + B z : Type)%type (at level 50, format "A  ∪  B", left associativity).
 
+Definition gax_at P := forall a, Forall atomic (projT2 (pgax P) a).
+Definition gax_cut P := forall a b x l1 l2 l3 l4,
+  projT2 (pgax P) a = (l1 ++ dual x :: l2) -> projT2 (pgax P) b = (l3 ++ x :: l4) ->
+  { c | projT2 (pgax P) c = l3 ++ l2 ++ l1 ++ l4 }.
+
 Lemma ex_app P : forall l1 l2, ll P (l1 ++ l2) -> ll P (l2 ++ l1).
 Proof. intros l1 l2 pi; eapply ex_r ; [ apply pi | apply PCperm_Type_app_comm ]. Qed.
+
+Section CutElim_At.
+
+  Variable P : pfrag.
+  Hypothesis P_gax_cut : gax_cut P.
+
+  Theorem cut_at : forall X l1 l2 l3 l4,
+    ll P (l1 ++ var X :: l2) -> ll P (l3 ++ covar X :: l4) -> ll P (l1 ++ l4 ++ l3 ++ l2).
+  Proof.
+  enough (forall s A l0 l1 l2 (pi1: ll P (A :: l0)) (pi2 : ll P (l1 ++ dual A :: l2)),
+         s = psize pi1 + psize pi2 -> { X & A = var X } + { X & A = covar X } -> ll P (l1 ++ l0 ++ l2))
+    as Hat.
+  { intros X l1 l2 l3 l4 pi1 pi2.
+    eapply ex_r; [ | apply PCperm_Type_app_comm ].
+    rewrite app_assoc; rewrite <- 2 app_assoc.
+    eapply ex_r; [ | apply PCperm_Type_app_comm ].
+    rewrite <- app_assoc.
+    apply (ex_r _ _ ((var X :: l2) ++ l1)) in pi1 ; [ | apply PCperm_Type_app_comm ].
+    rewrite <- app_comm_cons in pi1.
+    refine (Hat (psize pi1 + psize pi2) (var X) (l2 ++ l1) l3 l4 pi1 pi2 _ _).
+    - reflexivity.
+    - left; eexists; reflexivity. }
+  induction s as [s IHsize0] using lt_wf_rect; intros A l0 l1 l2 pi1 pi2 Heqs Hat; subst.
+  remember (l1 ++ dual A :: l2) as l; destruct_ll pi2 f X l Hl Hr HP a; simpl in IHsize0.
+  - destruct l1; inversion Heql; subst.
+    + apply codual in H0; simpl; subst.
+      eapply ex_r; [ | apply PCperm_Type_app_comm ].
+      apply pi1.
+    + destruct l1; inversion H1; [ | destruct l1; inversion H2 ]; subst.
+      apply codual in H0; simpl; subst.
+      list_simpl; apply pi1.
+  - apply PCperm_Type_vs_elt_inv in HP.
+    destruct HP as [(l1',l2') Heq HP']; subst.
+    apply (ex_r _ (l1' ++ l0 ++ l2')).
+    + refine (IHsize0 (psize pi1 + psize Hl) _ _ _ _ _ pi1 Hl _ Hat); try lia.
+    + etransitivity; [ apply PCperm_Type_app_comm | ].
+      etransitivity; [ | apply PCperm_Type_app_comm ].
+      list_simpl; symmetry.
+      apply PEperm_PCperm_Type.
+      apply PEperm_Type_app_head; assumption.
+  - trichot_Type_elt_app_exec Heql; subst.
+    + rewrite 2 app_assoc.
+      eapply ex_wn_r; [ | apply HP ].
+      revert Hl IHsize0; list_simpl; intros Hl IHsize0.
+      refine (IHsize0 (psize pi1 + psize Hl) _ _ _ _ _ pi1 Hl _ Hat); try lia.
+    + destruct Heql1 as [H _].
+      decomp_map_Type H.
+      destruct A; inversion H3; destruct Hat as [[? Heq] | [? Heq]]; inversion Heq.
+    + list_simpl.
+      eapply ex_wn_r; [ | apply HP ].
+      revert Hl IHsize0; rewrite 2 app_assoc; intros Hl IHsize0.
+      rewrite 2 app_assoc.
+      refine (IHsize0 (psize pi1 + psize Hl) _ _ _ _ _ pi1 Hl _ Hat); try lia.
+  - destruct l1; inversion Heql.
+  - dichot_Type_elt_app_exec Heql; subst.
+    + rewrite 2 app_assoc.
+      apply mix2_r; auto.
+      list_simpl.
+      refine (IHsize0 (psize pi1 + psize Hr) _ _ _ _ _ pi1 Hr _ Hat); try lia.
+    + list_simpl.
+      apply mix2_r; auto.
+      refine (IHsize0 (psize pi1 + psize Hl) _ _ _ _ _ pi1 Hl _ Hat); try lia.
+  - destruct l1; inversion Heql; [ | destruct l1; inversion H1 ].
+    destruct A; inversion H0.
+    destruct Hat as [[X Heq] | [X Heq]]; discriminate Heq.
+  - destruct l1; inversion Heql; subst.
+    + destruct A; inversion H0.
+      destruct Hat as [[X Heq] | [X Heq]]; discriminate Heq.
+    + simpl; apply bot_r.
+      refine (IHsize0 (psize pi1 + psize Hl) _ _ _ _ _ pi1 Hl _ Hat); try lia.
+  - destruct l1; inversion Heql; subst.
+    + destruct A; inversion H0.
+      destruct Hat as [[X Heq] | [X Heq]]; discriminate Heq.
+    + dichot_Type_elt_app_exec H1; subst.
+      * list_simpl; rewrite 2 app_assoc.
+        apply tens_r; auto.
+        list_simpl; rewrite app_comm_cons.
+        revert Hr IHsize0; rewrite app_comm_cons; intros Hr IHsize0.
+        refine (IHsize0 (psize pi1 + psize Hr) _ _ _ _ _ pi1 Hr _ Hat); try lia.
+      * list_simpl.
+        apply tens_r; auto.
+        list_simpl; rewrite app_comm_cons.
+        revert Hl IHsize0; rewrite app_comm_cons; intros Hl IHsize0.
+        refine (IHsize0 (psize pi1 + psize Hl) _ _ _ _ _ pi1 Hl _ Hat); try lia.
+  - destruct l1; inversion Heql; subst.
+    + destruct A; inversion H0.
+      destruct Hat as [[X Heq] | [X Heq]]; discriminate Heq.
+    + simpl; apply parr_r.
+      revert Hl IHsize0; rewrite 2 app_comm_cons; intros Hl IHsize0.
+      refine (IHsize0 (psize pi1 + psize Hl) _ _ _ _ _ pi1 Hl _ Hat); try lia.
+  - destruct l1; inversion Heql; subst.
+    + destruct A; inversion H0.
+      destruct Hat as [[X Heq] | [X Heq]]; discriminate Heq.
+    + apply top_r.
+  - destruct l1; inversion Heql; subst.
+    + destruct A; inversion H0.
+      destruct Hat as [[X Heq] | [X Heq]]; discriminate Heq.
+    + simpl; apply plus_r1.
+      revert Hl IHsize0; rewrite app_comm_cons; intros Hl IHsize0.
+      refine (IHsize0 (psize pi1 + psize Hl) _ _ _ _ _ pi1 Hl _ Hat); try lia.
+  - destruct l1; inversion Heql; subst.
+    + destruct A; inversion H0.
+      destruct Hat as [[X Heq] | [X Heq]]; discriminate Heq.
+    + simpl; apply plus_r2.
+      revert Hl IHsize0; rewrite app_comm_cons; intros Hl IHsize0.
+      refine (IHsize0 (psize pi1 + psize Hl) _ _ _ _ _ pi1 Hl _ Hat); try lia.
+  - destruct l1; inversion Heql; subst.
+    + destruct A; inversion H0.
+      destruct Hat as [[X Heq] | [X Heq]]; discriminate Heq.
+    + simpl; apply with_r.
+      * revert Hl IHsize0; rewrite app_comm_cons; intros Hl IHsize0.
+        refine (IHsize0 (psize pi1 + psize Hl) _ _ _ _ _ pi1 Hl _ Hat); try lia.
+      * revert Hr IHsize0; rewrite app_comm_cons; intros Hr IHsize0.
+        refine (IHsize0 (psize pi1 + psize Hr) _ _ _ _ _ pi1 Hr _ Hat); try lia.
+  - destruct l1; inversion Heql; subst.
+    + destruct A; inversion H0.
+      destruct Hat as [[X Heq] | [X Heq]]; discriminate Heq.
+    + symmetry in H1; decomp_map_Type H1.
+      destruct A; inversion H1.
+      destruct Hat as [[X Heq] | [X Heq]]; discriminate Heq.
+  -  destruct l1; inversion Heql; subst.
+    + destruct A; inversion H0.
+      destruct Hat as [[X Heq] | [X Heq]]; discriminate Heq.
+    + simpl; apply de_r.
+      revert Hl IHsize0; rewrite app_comm_cons; intros Hl IHsize0.
+      refine (IHsize0 (psize pi1 + psize Hl) _ _ _ _ _ pi1 Hl _ Hat); try lia.
+  - destruct l1; inversion Heql; subst.
+    + destruct A; inversion H0.
+      destruct Hat as [[X Heq] | [X Heq]]; discriminate Heq.
+    + simpl; apply wk_r.
+      refine (IHsize0 (psize pi1 + psize Hl) _ _ _ _ _ pi1 Hl _ Hat); try lia.
+  - destruct l1; inversion Heql; subst.
+    + destruct A; inversion H0.
+      destruct Hat as [[X Heq] | [X Heq]]; discriminate Heq.
+    + simpl; apply co_r.
+      revert Hl IHsize0; rewrite 2 app_comm_cons; intros Hl IHsize0.
+      refine (IHsize0 (psize pi1 + psize Hl) _ _ _ _ _ pi1 Hl _ Hat); try lia.
+  - dichot_Type_elt_app_exec Heql; subst.
+    + rewrite 2 app_assoc.
+      eapply (cut_r _ A0); auto.
+      list_simpl; rewrite app_comm_cons.
+      revert Hr IHsize0; rewrite app_comm_cons; intros Hr IHsize0.
+      refine (IHsize0 (psize pi1 + psize Hr) _ _ _ _ _ pi1 Hr _ Hat); try lia.
+    + list_simpl.
+      eapply (cut_r _ A0); auto.
+      list_simpl; rewrite app_comm_cons.
+      revert Hl IHsize0; rewrite app_comm_cons; intros Hl IHsize0.
+      refine (IHsize0 (psize pi1 + psize Hl) _ _ _ _ _ pi1 Hl _ Hat); try lia.
+    Unshelve. all: auto.
+  - clear IHsize0.
+    remember (A :: l0) as l.
+    rewrite <- (app_nil_l l2) ; rewrite <- (app_nil_l (A :: l0)) in Heql0.
+    remember nil as l3 ; clear Heql3.
+    revert l3 l0 Heql0 ; induction pi1 ; intros l4 l5 Heq ; subst.
+    + destruct l4 ; inversion Heq ; subst.
+      * simpl in Heql; list_simpl ; rewrite <- Heql ; apply (gax_r _ a).
+      * destruct l4 ; inversion H1 ; subst.
+        -- simpl in Heql; list_simpl ; rewrite <- Heql ; apply (gax_r _ a).
+        -- destruct l4 ; inversion H2.
+    + apply PCperm_Type_vs_elt_inv in p.
+      destruct p as [[l4' l5'] Heq p] ; simpl in Heq ; simpl in p ; subst.
+      assert (PEperm_Type (pperm P) (l1 ++ l5' ++ l4' ++ l2) (l1 ++ l5 ++ l4 ++ l2)) as HP'.
+      { apply PEperm_Type_app_head.
+        rewrite 2 app_assoc ; apply PEperm_Type_app_tail.
+        symmetry; assumption. }
+      apply PEperm_PCperm_Type in HP'.
+      apply (ex_r _ (l1 ++ l5' ++ l4' ++ l2))...
+      apply IHpi1; try reflexivity.
+      apply PEperm_PCperm_Type.
+      symmetry.
+      apply PEperm_Type_app_head.
+      rewrite 2 (app_assoc _ _ l2).
+      apply PEperm_Type_app_tail; assumption.
+    + symmetry in Heq ; trichot_Type_elt_app_exec Heq ; subst.
+      * list_simpl ; rewrite app_assoc.
+        eapply ex_wn_r; try eassumption.
+        list_simpl.
+        rewrite (app_assoc l) ; rewrite (app_assoc _ l3) ; rewrite <- (app_assoc l).
+        apply IHpi1 ; list_simpl; reflexivity.
+      * destruct Heq1 as [Heq1 Heq2] ; decomp_map_Type Heq1.
+        exfalso ; destruct A ; inversion Heq1 ; subst ; destruct Hat as [[? Heq] | [? Heq]]; discriminate Heq.
+      * list_simpl ; rewrite 2 app_assoc.
+        eapply ex_wn_r; try eassumption.
+        list_simpl ; rewrite (app_assoc l0) ; rewrite (app_assoc _ l6).
+        apply IHpi1 ; list_simpl; reflexivity.
+    + destruct l4 ; inversion Heq.
+    + dichot_Type_elt_app_exec Heq ; subst.
+      * list_simpl.
+        eapply ex_r ; [ | apply PCperm_Type_app_rot ] ; list_simpl.
+        apply mix2_r; auto.
+        eapply ex_r ; [ | apply PCperm_Type_app_rot ] ; list_simpl.
+        apply IHpi1_2 ; list_simpl; reflexivity.
+      * eapply ex_r ; [ | apply PCperm_Type_app_rot ] ; list_simpl.
+        apply mix2_r; auto.
+        eapply ex_r ; [ | apply PCperm_Type_app_rot ] ; list_simpl.
+        apply IHpi1_1 ; list_simpl; reflexivity.
+    + exfalso ; destruct l4 ; inversion Heq.
+      * destruct A ; inversion H0 ; subst ; destruct Hat as [[? Heq'] | [? Heq']]; discriminate Heq'.
+      * destruct l4 ; inversion H1.
+    + destruct l4 ; inversion Heq ; subst ;
+        try (exfalso ; destruct Hat as [[? Heq'] | [? Heq']]; discriminate Heq'; fail).
+      eapply ex_r ; [ | apply PCperm_Type_app_rot ] ; list_simpl.
+      apply bot_r.
+      eapply ex_r ; [ | apply PCperm_Type_app_rot ] ; list_simpl.
+      apply IHpi1 ; list_simpl; reflexivity.
+    + destruct l4 ; inversion Heq ; subst ;
+        try (exfalso ; destruct Hat as [[? Heq'] | [? Heq']]; discriminate Heq'; fail).
+      dichot_Type_elt_app_exec H1 ; subst.
+      * list_simpl.
+        eapply ex_r ; [ | apply PCperm_Type_app_rot ] ; list_simpl.
+        rewrite app_comm_cons ; eapply ex_r ; [ | symmetry ; apply PCperm_Type_app_rot ] ; list_simpl.
+        rewrite 3 app_assoc ; apply tens_r; try assumption.
+        list_simpl ; rewrite app_comm_cons ; eapply ex_r ; [ | apply PCperm_Type_app_rot ] ; list_simpl.
+        rewrite app_comm_cons ; apply IHpi1_2 ; list_simpl; reflexivity.
+      * eapply ex_r ; [ | apply PCperm_Type_app_rot ] ; list_simpl.
+        apply tens_r; try assumption.
+        list_simpl ; rewrite app_comm_cons ; eapply ex_r ; [ | apply PCperm_Type_app_rot ] ; list_simpl.
+        rewrite app_comm_cons ; apply IHpi1_1 ; list_simpl; reflexivity.
+    + destruct l4 ; inversion Heq ; subst ;
+        try (exfalso ; destruct Hat as [[? Heq'] | [? Heq']]; discriminate Heq'; fail).
+      eapply ex_r ; [ | apply PCperm_Type_app_rot ] ; list_simpl.
+      apply parr_r.
+      rewrite 2 app_comm_cons ; eapply ex_r ; [ | apply PCperm_Type_app_rot ] ; list_simpl.
+      rewrite 2 app_comm_cons ; apply IHpi1 ; list_simpl; reflexivity.
+    + destruct l4 ; inversion Heq ; subst ;
+        try (exfalso ; destruct Hat as [[? Heq'] | [? Heq']]; discriminate Heq'; fail).
+      eapply ex_r ; [ | apply PCperm_Type_app_rot ] ; list_simpl.
+      apply top_r...
+    + destruct l4 ; inversion Heq ; subst ;
+        try (exfalso ; destruct Hat as [[? Heq'] | [? Heq']]; discriminate Heq'; fail).
+      eapply ex_r ; [ | apply PCperm_Type_app_rot ] ; list_simpl.
+      apply plus_r1...
+      rewrite app_comm_cons ; eapply ex_r ; [ | apply PCperm_Type_app_rot ] ; list_simpl.
+      rewrite app_comm_cons ; apply IHpi1 ; list_simpl; reflexivity.
+    + destruct l4 ; inversion Heq ; subst ;
+        try (exfalso ; destruct Hat as [[? Heq'] | [? Heq']]; discriminate Heq'; fail).
+      eapply ex_r ; [ | apply PCperm_Type_app_rot ] ; list_simpl.
+      apply plus_r2.
+      rewrite app_comm_cons ; eapply ex_r ; [ | apply PCperm_Type_app_rot ] ; list_simpl.
+      rewrite app_comm_cons ; apply IHpi1 ; list_simpl; reflexivity.
+    + destruct l4 ; inversion Heq ; subst ;
+        try (exfalso ; destruct Hat as [[? Heq'] | [? Heq']]; discriminate Heq'; fail).
+      eapply ex_r ; [ | apply PCperm_Type_app_rot ] ; list_simpl.
+      apply with_r.
+      * rewrite app_comm_cons ; eapply ex_r ; [ | apply PCperm_Type_app_rot ] ; list_simpl.
+        rewrite app_comm_cons ; apply IHpi1_1 ; list_simpl; reflexivity.
+      * rewrite app_comm_cons ; eapply ex_r ; [ | apply PCperm_Type_app_rot ] ; list_simpl.
+        rewrite app_comm_cons ; apply IHpi1_2 ; list_simpl; reflexivity.
+    + destruct l4 ; inversion Heq ; subst ;
+        try (exfalso ; destruct Hat as [[? Heq'] | [? Heq']]; discriminate Heq'; fail).
+      exfalso ; symmetry in H1 ; decomp_map_Type H1 ; destruct A ; inversion H1 ; subst ;
+        destruct Hat as [[? Heq'] | [? Heq']]; discriminate Heq'.
+    + destruct l4 ; inversion Heq ; subst ;
+        try (exfalso ; destruct Hat as [[? Heq'] | [? Heq']]; discriminate Heq'; fail).
+      eapply ex_r ; [ | apply PCperm_Type_app_rot ] ; list_simpl.
+      apply de_r.
+      rewrite app_comm_cons ; eapply ex_r ; [ | apply PCperm_Type_app_rot ] ; list_simpl.
+      rewrite app_comm_cons ; apply IHpi1 ; list_simpl; reflexivity.
+    + destruct l4 ; inversion Heq ; subst ;
+        try (exfalso ; destruct Hat as [[? Heq'] | [? Heq']]; discriminate Heq'; fail).
+      eapply ex_r ; [ | apply PCperm_Type_app_rot ] ; list_simpl.
+      apply wk_r.
+      eapply ex_r ; [ | apply PCperm_Type_app_rot ] ; list_simpl.
+      apply IHpi1 ; list_simpl; reflexivity.
+    + destruct l4 ; inversion Heq ; subst ;
+        try (exfalso ; destruct Hat as [[? Heq'] | [? Heq']]; discriminate Heq'; fail).
+      eapply ex_r ; [ | apply PCperm_Type_app_rot ] ; list_simpl.
+      apply co_r.
+      rewrite 2 app_comm_cons ; eapply ex_r ; [ | apply PCperm_Type_app_rot ] ; list_simpl.
+      rewrite 2 app_comm_cons ; apply IHpi1 ; list_simpl; reflexivity.
+    + dichot_Type_elt_app_exec Heq; subst.
+      * apply (ex_r _ (l0 ++ l4 ++ l2 ++ l1 ++ l)).
+        -- eapply (cut_r _ (dual A0)); try rewrite bidual; auto.
+           apply (ex_r _ ((l2 ++ l1) ++ l ++ A0 :: l4)).
+           ++ eapply (cut_r _ (dual A)); try rewrite bidual.
+              ** eapply ex_r; [ apply pi1_2 | ].
+                 rewrite 2 app_comm_cons; apply PCperm_Type_app_comm.
+              ** eapply ex_r; [ apply (gax_r _ a) | ].
+                 rewrite Heql.
+                 rewrite app_comm_cons; apply PCperm_Type_app_comm.
+           ++ rewrite app_comm_cons.
+              etransitivity; [ | apply PCperm_Type_app_comm ]; list_simpl; reflexivity.
+        -- rewrite 2 app_assoc.
+           etransitivity; [ apply PCperm_Type_app_comm | ]; list_simpl; reflexivity.
+      * apply (ex_r _ (l3 ++ l6 ++ l2 ++ l1 ++ l5)).
+        -- eapply (cut_r _ A0); auto.
+           apply (ex_r _ ((l2 ++ l1) ++ l5 ++ dual A0 :: l6)).
+           ++ eapply (cut_r _ (dual A)); try rewrite bidual.
+              ** eapply ex_r; [ apply pi1_1 | ].
+                 rewrite 2 app_comm_cons; apply PCperm_Type_app_comm.
+              ** eapply ex_r; [ apply (gax_r _ a) | ].
+                 rewrite Heql.
+                 rewrite app_comm_cons; apply PCperm_Type_app_comm.
+           ++ rewrite app_comm_cons.
+              etransitivity; [ | apply PCperm_Type_app_comm ]; list_simpl; reflexivity.
+        -- rewrite 2 app_assoc.
+           etransitivity; [ apply PCperm_Type_app_comm | ]; list_simpl; reflexivity.
+      Unshelve. all: auto.
+    + destruct (P_gax_cut _ _ _ _ _ _ _ Heql Heq) as [x Hcut].
+      apply (ex_r _ (l4 ++ l2 ++ l1 ++ l5)).
+      * rewrite <- Hcut ; apply (gax_r _ x).
+      * rewrite app_assoc.
+        rewrite (app_assoc _ _ (l4 ++ _)).
+        apply PCperm_Type_app_comm.
+  Qed.
+
+End CutElim_At.
 
 Global Instance CPS_ctx P : CPhaseSpace (pperm P) (pmix0 P) (pmix2 P).
 Proof.
@@ -58,7 +371,9 @@ Defined.
 Section Okada.
 
   Context { P : pfrag }.
-  Hypothesis Pgax : projT1 (pgax P) -> False.
+
+  Hypothesis P_gax_at : gax_at P.
+  Hypothesis P_gax_cut : gax_cut P.
 
   Notation "↓" := (fun A Γ => ll P (A::Γ)).
 
@@ -66,17 +381,69 @@ Section Okada.
 
   Instance CPSLL : CPhaseSpace (pperm P) (pmix0 P) (pmix2 P) := CPS_ctx P.
 
+  Infix "∘" := (MComposes CPSCompose) (at level 50, no associativity).
+  Notation dual := (ldual (R CPSCompose CPSPole)).
+  Notation "'⟦' A '⟧'" := (@Form_sem (pperm P) (pmix0 P) (pmix2 P) _ LLval A) (at level 49).
+  Notation "⟬߭  ll ⟭" := (@list_Form_presem (pperm P) (pmix0 P) (pmix2 P) _ LLval ll) (at level 49).
+
+  Hint Resolve (@CPSfact_pole _ _ _ CPSLL) (@CPScommute _ _ _ CPSLL)
+               CPSassociative_l CPSassociative_r
+               CPSneutral_1 CPSneutral_2
+               CPSneutral_l_1 CPSneutral_l_2 CPSneutral_r_1 CPSneutral_r_2.
+
+  Fact LLgax : forall a, ⟬߭  projT2 (pgax P) a ⟭ ⊆ CPSPole.
+  Proof.
+  intros a; red in P_gax_at; specialize P_gax_at with a.
+  assert (pi := gax_r _ a).
+  remember (projT2 (pgax P) a) as l; clear Heql a.
+  enough (forall l, Forall atomic l -> forall l0, ll P (l0 ++ l) -> sg l0 ∘ ⟬߭ l ⟭  ⊆ CPSPole) as IH.
+  { specialize IH with l nil.
+    etransitivity; [ | apply CPSfact_pole ].
+    apply subset_cl.
+    etransitivity; [ apply (@neutral_l_1_g _ _ CPSUnit _ CPScommute) | ]; auto.
+    apply cl_subset.
+    etransitivity; [ apply stability_r | ]; auto.
+    apply cl_subset.
+    etransitivity; [ | apply cl_increase ].
+    etransitivity; [ | apply IH ]; auto.
+    apply MComposes_monotone; try reflexivity. }
+  clear pi P_gax_at.
+  induction l0; intros HF l1 pi; intros x Hx; inversion Hx; rewrite_all <- H.
+  - inversion X.
+    apply pi.
+  - inversion X; simpl.
+    eapply ex_r; [ | apply PCperm_Type_app_comm ]; rewrite <- app_assoc.
+    apply X0.
+    destruct a; try (exfalso; inversion HF; inversion H4; fail); subst; simpl.
+    + change (var a :: y0 ++ x0) with ((var a :: nil) ++ y0 ++ x0).
+      rewrite app_assoc; eapply ex_r; [ | apply PCperm_Type_app_comm ]; rewrite app_assoc.
+      specialize IHl0 with (x0 ++ var a :: nil).
+      apply IHl0.
+      * clear - HF; inversion HF; assumption.
+      * list_simpl; assumption.
+      * constructor; auto.
+    + intros y Hy; red.
+      rewrite <- app_assoc.
+      eapply ex_r; [ | apply PCperm_Type_app_comm ].
+      specialize IHl0 with (x0 ++ y).
+      apply IHl0.
+      * clear - HF; inversion HF; assumption.
+      * eapply ex_r; [ | apply PCperm_Type_app_comm ].
+        rewrite <- (app_nil_l _).
+        rewrite <- (app_nil_l _) in Hy.
+        eapply cut_at; eassumption.
+      * constructor; auto.
+  Qed.
+
   Instance PMLL : CPhaseModel P.
   Proof. split with CPSLL LLval.
   intros X l H; simpl in H; red in H; red in H.
   eapply ex_r ; [ apply (H (var X :: nil)) | ].
   - intros l' pi; assumption.
   - etransitivity; [ apply PCperm_Type_app_comm | ]; reflexivity.
+  - apply LLgax.
   Defined.
 
-  Notation dual := (ldual (R CPSCompose CPSPole)).
-  Notation "'⟦' A '⟧'" := (@Form_sem (pperm P) (pmix0 P) (pmix2 P) _ LLval A) (at level 49).
-  Notation "⟬߭  ll ⟭" := (@list_Form_presem (pperm P) (pmix0 P) (pmix2 P) _ LLval ll) (at level 49).
 
   Lemma Okada A : ⟦A⟧ ⊆ ↓A.
   Proof.
@@ -142,7 +509,8 @@ End Okada.
 Section Cut_Elim.
 
   Context { P : pfrag }.
-  Hypothesis Pgax : projT1 (pgax P) -> False.
+  Hypothesis P_gax_at : gax_at P.
+  Hypothesis P_gax_cut : gax_cut P.
 
   Notation "↓" := (fun A Γ => ll (cutupd_pfrag P false) (A::Γ)).
   Notation LLval_cf := (fun x => ↓(var x)).
@@ -155,6 +523,7 @@ Section Cut_Elim.
   eapply ex_r ; [ apply (H (var X :: nil)) | ].
   - intros l' pi; assumption.
   - etransitivity; [ apply PCperm_Type_app_comm | ]; reflexivity.
+  - apply (@LLgax (cutupd_pfrag P false) P_gax_at P_gax_cut).
   Defined.
 
   Theorem ll_cut_elimination Γ : ll P Γ -> ll (cutupd_pfrag P false) Γ.
